capDL: introduce generic page tables
- Drawing inspiration from AARCH64, make page table object and cap types
  parametric in pt_type. This means we need only one PageTable
  type for all page table objects (page directory, page table, etc), and
  only one page table cap type to point to them.

- Use the same type/level distinction as in AARCH64, because it can
  model all situations that occur in the currently supported seL4
  architectures. In particular, all levels could use the same type
  such as in RISCV64, each level could use its own type such as for
  X64/ARM/ARM_HYP, or a mix as in AARCH64.

- Update the existing ARM/ARM_HYP capDL spec to use this scheme.

- Add a generic implementation of page tables that works for all seL4
  architectures. It only implements "map" system calls, returning
  maximum nondeterminism otherwise. That means, other system calls will
  not be usable in capDL. However, "map" is the only page/page table
  invocation that is needed in system initialisation.

- Keep the old ARM/ARM_HYP implementation and call it when the
  architecture is AARCH32 to keep the current DRefine/SysInit proofs
  (mostly) working. The proofs will need updates for the new data types
  being used, but the existing reasoning will still apply.

Signed-off-by: Gerwin Klein <gerwin.klein@proofcraft.systems>

spec/capDL/AARCH64/Arch_Structs_D.thy
@@ -35,13 +35,25 @@ context Arch begin arch_global_naming
 
 lemmas vmpage_size_simps = vmpage_size.simps
 
+definition pageForPageBits :: "nat \<Rightarrow> vmpage_size" where
+  "pageForPageBits bits \<equiv>
+     if bits = pageBits then ARMSmallPage
+     else if bits = pageBits + ptTranslationBits NormalPT_T then ARMLargePage
+     else if bits = pageBits + 2 * ptTranslationBits NormalPT_T then ARMHugePage
+     else undefined"
+
+lemma pageForPageBits_pageBitsForSize[simp]:
+  "pageForPageBits (pageBitsForSize sz) = sz"
+  unfolding pageForPageBits_def pageBitsForSize_def
+  by (cases sz; simp add: ptTranslationBits_def)
+
+definition pt_size_index :: nat where
+  "pt_size_index \<equiv> 9"
+
 (* These names are expected by other architectures, but unused for AARCH64 *)
 
 definition pd_size_index :: nat where
   "pd_size_index \<equiv> undefined"
-
-definition pt_size_index :: nat where
-  "pt_size_index \<equiv> undefined"
 
 definition smallPageBits :: nat where
   "smallPageBits = undefined"
@@ -57,9 +69,6 @@ definition superSectionBits :: nat where
 
 definition pt_slot_vaddr_mask :: machine_word where
   "pt_slot_vaddr_mask = undefined"
-
-definition pageForPageBits :: "nat \<Rightarrow> vmpage_size" where
-  "pageForPageBits bits \<equiv> undefined"
 
 end
 end
